update indinvs

src/ra/IndexedInvariants.v
@@ -13,10 +13,10 @@ Section INDEXED_INVARIANT_SET.
   Class IInvSet (Vars : index -> Type) :=
     { prop : forall (i : index), (Vars i) -> iProp }.
 
-  Class IInvIn {Vars : index -> Type} `{IInvSet Vars} (n : index) (P : iProp) :=
-    { inhabitant : Vars n
-    ; inhabitant_eq : prop _ inhabitant = P
-    }.
+  (* Class IInvIn {Vars : index -> Type} `{IInvSet Vars} (n : index) (P : iProp) := *)
+  (*   { inhabitant : Vars n *)
+  (*   ; inhabitant_eq : prop _ inhabitant = P *)
+  (*   }. *)
 
   Definition InvSetRA (Vars : index -> Type) (n : index) : URA.t :=
     (Auth.t (positive ==> URA.agree (Vars n)))%ra.
@@ -622,8 +622,8 @@ Section FANCY_UPDATE.
   Context `{@GRA.inG (index ==> Gset.t)%ra Σ}.
   Context `{@GRA.inG (IInvSetRA Vars) Σ}.
 
-  Definition inv (n : index) (N : namespace) P :=
-    (∃ p, ∃ i, ⌜prop n p = P⌝ ∧ ⌜i ∈ (↑N : coPset)⌝ ∧ OwnI n i p)%I.
+  Definition inv (n : index) (N : namespace) p :=
+    (∃ i, ⌜i ∈ (↑N : coPset)⌝ ∧ OwnI n i p)%I.
 
   Definition FUpd x (A : iProp) (Es1 Es2 : coPsets) (P : iProp) : iProp :=
     A ∗ wsats x ∗ OwnEs Es1 -∗ #=> (A ∗ wsats x ∗ OwnEs Es2 ∗ P).
@@ -638,20 +638,22 @@ Section FANCY_UPDATE.
     iModIntro. iFrame. iApply wsats_nin. apply LT. iFrame.
   Qed.
 
-  Lemma FUpd_alloc x A Es n N P `{hasP : @IInvIn Σ Vars Invs n P} :
-    n < x -> P ⊢ FUpd x A Es Es (inv n N P).
+  Lemma FUpd_alloc x A Es n N p :
+    n < x -> prop n p ⊢ FUpd x A Es Es (inv n N p).
   Proof.
-    destruct hasP as [p HE]. subst. iIntros (LT) "P (A & WSAT & EN)".
+    iIntros (LT) "P (A & WSAT & EN)".
     iMod (wsats_OwnI_alloc_lt _ _ LT p (fun i => i ∈ ↑N) with "[WSAT P]") as "[I WSAT]".
     - i. des_ifs. apply iris.base_logic.lib.invariants.fresh_inv_name.
     - iFrame.
-    - iModIntro. iFrame. iDestruct "I" as "[% I]". iExists p, i. iFrame. ss.
+    - iModIntro. iFrame.
   Qed.
 
-  Lemma FUpd_open_aux x A Es n N E (LT : n < x) (INE : Es !! n = Some E) (IN : ↑N ⊆ E) P :
-    inv n N P ⊢ FUpd x A Es (<[n := E∖↑N]> Es) (P ∗ (P -∗ FUpd x A (<[n := E∖↑N]> Es) Es emp)).
+  Lemma FUpd_open_aux x A Es n N E (LT : n < x) (INE : Es !! n = Some E) (IN : ↑N ⊆ E) p :
+    inv n N p ⊢
+        FUpd x A Es (<[n := E∖↑N]> Es)
+        ((prop n p) ∗ ((prop n p) -∗ FUpd x A (<[n := E∖↑N]> Es) Es emp)).
   Proof.
-    iIntros "[% [% (%HP & %iN & #HI)]] (A & WSAT & ENS)". subst.
+    iIntros "[% (%iN & #HI)] (A & WSAT & ENS)".
     iPoseProof ((OwnEs_acc_in _ _ _ INE) with "ENS") as "[EN ENS]".
     iAssert (OwnE n (E ∖ ↑N) ∗ OwnE n (↑N ∖ {[i]}) ∗ OwnE n {[i]})%I with "[EN]" as "(EN1 & EN2 & EN3)".
     { iApply bi.sep_mono_r.
@@ -679,13 +681,13 @@ Section FANCY_UPDATE.
     rewrite difference_union_L. set_solver.
   Qed.
 
-  Lemma FUpd_open x A Es n N (LT : n < x) (IN : subseteq_def Es n (↑N)) P :
-    inv n N P ⊢
+  Lemma FUpd_open x A Es n N (LT : n < x) (IN : subseteq_def Es n (↑N)) p :
+    inv n N p ⊢
         FUpd x A Es
         (<[n := (lookup_def Es n)∖↑N]> Es)
-        (P ∗ (P -∗ FUpd x A (<[n := (lookup_def Es n)∖↑N]> Es) Es emp)).
+        ((prop n p) ∗ ((prop n p) -∗ FUpd x A (<[n := (lookup_def Es n)∖↑N]> Es) Es emp)).
   Proof.
-    iIntros "[% [% (%HP & %iN & #HI)]] (A & WSAT & ENS)". subst.
+    iIntros "[% (%iN & #HI)] (A & WSAT & ENS)".
     unfold lookup_def, subseteq_def in *. destruct (Es !! n) eqn:CASES; ss.
     - iApply FUpd_open_aux; auto. unfold inv; auto. iFrame.
     - iAssert (
@@ -857,11 +859,11 @@ Use [FUpd_mask_frame] and [FUpd_intro_mask]")
     iApply "Hfin". iFrame.
   Qed.
 
-  Global Instance into_acc_FUpd_inv x A Es n N P :
-    IntoAcc (inv n N P) (n < x /\ subseteq_def Es n (↑N)) True
+  Global Instance into_acc_FUpd_inv x A Es n N p :
+    IntoAcc (inv n N p) (n < x /\ subseteq_def Es n (↑N)) True
             (FUpd x A Es (<[n := lookup_def Es n ∖ ↑N]>Es))
             (FUpd x A (<[n := lookup_def Es n ∖ ↑N]>Es) Es)
-            (fun _ : () => P) (fun _ : () => P) (fun _ : () => None).
+            (fun _ : () => prop n p) (fun _ : () => prop n p) (fun _ : () => None).
   Proof.
     rewrite /IntoAcc. iIntros ((LT & iE)) "INV _". rewrite /accessor.
     iPoseProof (FUpd_open _ _ _ _ _ LT iE with "INV") as ">[open close]".
@@ -879,6 +881,273 @@ Use [FUpd_mask_frame] and [FUpd_intro_mask]")
 End FANCY_UPDATE.
 
 Global Opaque FUpd.
+
+(* Section FANCY_UPDATE. *)
+
+(*   Context `{Σ : GRA.t}. *)
+(*   Context `{Vars : index -> Type}. *)
+(*   Context `{Invs : @IInvSet Σ Vars}. *)
+(*   Context `{@GRA.inG (index ==> CoPset.t)%ra Σ}. *)
+(*   Context `{@GRA.inG (index ==> Gset.t)%ra Σ}. *)
+(*   Context `{@GRA.inG (IInvSetRA Vars) Σ}. *)
+
+(*   Definition inv (n : index) (N : namespace) P := *)
+(*     (∃ p, ∃ i, ⌜prop n p = P⌝ ∧ ⌜i ∈ (↑N : coPset)⌝ ∧ OwnI n i p)%I. *)
+
+(*   Definition FUpd x (A : iProp) (Es1 Es2 : coPsets) (P : iProp) : iProp := *)
+(*     A ∗ wsats x ∗ OwnEs Es1 -∗ #=> (A ∗ wsats x ∗ OwnEs Es2 ∗ P). *)
+
+
+(*   Lemma FUpd_mono x0 x1 A Es1 Es2 P : *)
+(*     (x0 < x1) -> FUpd x0 A Es1 Es2 P ⊢ FUpd x1 A Es1 Es2 P. *)
+(*   Proof. *)
+(*     iIntros (LT) "FUPD (A & SAT & EN)". *)
+(*     iPoseProof ((wsats_in _ _ LT) with "SAT") as "[SAT K]". *)
+(*     iMod ("FUPD" with "[A SAT EN]") as "(A & SAT & EN & P)". iFrame. *)
+(*     iModIntro. iFrame. iApply wsats_nin. apply LT. iFrame. *)
+(*   Qed. *)
+
+(*   Lemma FUpd_alloc x A Es n N P `{hasP : @IInvIn Σ Vars Invs n P} : *)
+(*     n < x -> P ⊢ FUpd x A Es Es (inv n N P). *)
+(*   Proof. *)
+(*     destruct hasP as [p HE]. subst. iIntros (LT) "P (A & WSAT & EN)". *)
+(*     iMod (wsats_OwnI_alloc_lt _ _ LT p (fun i => i ∈ ↑N) with "[WSAT P]") as "[I WSAT]". *)
+(*     - i. des_ifs. apply iris.base_logic.lib.invariants.fresh_inv_name. *)
+(*     - iFrame. *)
+(*     - iModIntro. iFrame. iDestruct "I" as "[% I]". iExists p, i. iFrame. ss. *)
+(*   Qed. *)
+
+(*   Lemma FUpd_open_aux x A Es n N E (LT : n < x) (INE : Es !! n = Some E) (IN : ↑N ⊆ E) P : *)
+(*     inv n N P ⊢ FUpd x A Es (<[n := E∖↑N]> Es) (P ∗ (P -∗ FUpd x A (<[n := E∖↑N]> Es) Es emp)). *)
+(*   Proof. *)
+(*     iIntros "[% [% (%HP & %iN & #HI)]] (A & WSAT & ENS)". subst. *)
+(*     iPoseProof ((OwnEs_acc_in _ _ _ INE) with "ENS") as "[EN ENS]". *)
+(*     iAssert (OwnE n (E ∖ ↑N) ∗ OwnE n (↑N ∖ {[i]}) ∗ OwnE n {[i]})%I with "[EN]" as "(EN1 & EN2 & EN3)". *)
+(*     { iApply bi.sep_mono_r. *)
+(*       { apply OwnE_disjoint. set_solver. } *)
+(*       iApply OwnE_disjoint. *)
+(*       { set_solver. } *)
+(*       replace (E ∖ ↑N ∪ (↑N ∖ {[i]} ∪ {[i]})) with E. *)
+(*       - iFrame. *)
+(*       - transitivity ({[i]} ∪ ↑N ∖ {[i]} ∪ E ∖ ↑N). *)
+(*         + rewrite <- union_difference_singleton_L; ss. eapply union_difference_L; ss. *)
+(*         + rewrite union_comm_L. f_equal. rewrite union_comm_L. ss. *)
+(*     } *)
+(*     iMod (wsats_OwnI_open x n i p LT with "[HI WSAT EN3]") as "(P & WSAT & DIS)". *)
+(*     { iFrame. auto. } *)
+(*     iModIntro. iFrame. iPoseProof (OwnEs_union with "[ENS EN1]") as "ENS". iFrame. *)
+(*     replace (∅ ∪ E ∖ ↑N) with (E ∖ ↑N). 2: set_solver. *)
+(*     iFrame. iIntros "P (A & WSAT & EN1)". *)
+(*     iMod (wsats_OwnI_close x n i p LT with "[HI WSAT P DIS]") as "(WSAT & EN3)". *)
+(*     { iFrame. auto. } *)
+(*     iModIntro. iFrame. iSplit; auto. *)
+(*     iPoseProof (OwnE_union with "[EN2 EN3]") as "EN2". iFrame. *)
+(*     rewrite <- union_difference_singleton_L; ss. *)
+(*     iPoseProof (OwnEs_union with "[EN1 EN2]") as "ENS". iFrame. *)
+(*     rewrite insert_id. iFrame. rewrite INE. f_equal. *)
+(*     rewrite difference_union_L. set_solver. *)
+(*   Qed. *)
+
+(*   Lemma FUpd_open x A Es n N (LT : n < x) (IN : subseteq_def Es n (↑N)) P : *)
+(*     inv n N P ⊢ *)
+(*         FUpd x A Es *)
+(*         (<[n := (lookup_def Es n)∖↑N]> Es) *)
+(*         (P ∗ (P -∗ FUpd x A (<[n := (lookup_def Es n)∖↑N]> Es) Es emp)). *)
+(*   Proof. *)
+(*     iIntros "[% [% (%HP & %iN & #HI)]] (A & WSAT & ENS)". subst. *)
+(*     unfold lookup_def, subseteq_def in *. destruct (Es !! n) eqn:CASES; ss. *)
+(*     - iApply FUpd_open_aux; auto. unfold inv; auto. iFrame. *)
+(*     - iAssert ( *)
+(*           (#=> (A ∗ (wsats x ∗ (OwnEs (<[n:=⊤ ∖ ↑N]> Es) ∗ (prop n p ∗ (prop n p -∗ FUpd x A (<[n:=⊤ ∖ ↑N]> Es) (<[n:=⊤]>Es) emp)))))) *)
+(*             -∗ *)
+(*             #=> (A ∗ (wsats x ∗ (OwnEs (<[n:=⊤ ∖ ↑N]> Es) ∗ (prop n p ∗ (prop n p -∗ FUpd x A (<[n:=⊤ ∖ ↑N]> Es) Es emp))))))%I as "K". *)
+(*       { iIntros ">[A [SAT [ENS [P K]]]]". iModIntro. iFrame. iIntros "P". *)
+(*         iPoseProof ("K" with "P") as "K". iIntros "[A [SAT ENS]]". *)
+(*         iPoseProof ("K" with "[A SAT ENS]") as ">[A [SAT [ENS _]]]". iFrame. *)
+(*         iMod (OwnEs_free with "ENS") as "ENS". auto. *)
+(*         iModIntro. iFrame. *)
+(*       } *)
+(*       iApply "K". iClear "K". *)
+(*       iMod (OwnEs_alloc _ _ CASES with "ENS") as "ENS". remember (<[n:=⊤]> Es) as Es'. *)
+(*       replace (<[n:=⊤ ∖ ↑N]> Es) with (<[n:=⊤ ∖ ↑N]> Es'). *)
+(*       2:{ subst. rewrite insert_insert. auto. } *)
+(*       iApply FUpd_open_aux; auto. *)
+(*       { subst. apply lookup_insert. } *)
+(*       unfold inv; auto. iFrame. *)
+(*   Qed. *)
+
+(*   Lemma FUpd_intro x A Es P : *)
+(*     #=> P ⊢ FUpd x A Es Es P. *)
+(*   Proof. *)
+(*     iIntros "P H". iMod "P". iModIntro. iFrame. iFrame. *)
+(*   Qed. *)
+
+(*   Lemma FUpd_mask_frame_gen x A Es1 Es2 n E P : *)
+(*     (lookup_def Es1 n) ## E -> *)
+(*     FUpd x A Es1 Es2 P ⊢ *)
+(*          FUpd x A (<[n := (lookup_def Es1 n) ∪ E]>Es1) (<[n := (lookup_def Es2 n) ∪ E]>Es2) P. *)
+(*   Proof. *)
+(*     rewrite /FUpd. iIntros (D) "H (A & WSAT & ENS)". *)
+(*     iPoseProof ((OwnEs_acc_in _ n) with "ENS") as "[EN ENS]". apply lookup_insert. *)
+(*     iPoseProof (OwnE_disjoint _ _ _ D with "EN") as "[EN1 EN]". *)
+(*     iPoseProof (OwnEs_union with "[ENS EN1]") as "ENS". iFrame. *)
+(*     replace (∅ ∪ lookup_def Es1 n) with (lookup_def Es1 n) by set_solver. *)
+(*     destruct (coPset_equiv_dec E ∅); cycle 1. *)
+(*     { unfold lookup_def, default in D. des_ifs; ss. *)
+(*       2:{ exfalso. set_solver. } *)
+(*       rewrite insert_insert. rewrite (insert_id Es1). *)
+(*       2:{ unfold lookup_def, default. rewrite Heq. ss. } *)
+(*       iPoseProof ("H" with "[A WSAT ENS]") as ">(A & WSAT & ENS2 & P)". iFrame. *)
+(*       destruct (Es2 !! n) eqn:CASES. *)
+(*       2:{ iMod ((OwnEs_acc_new _ _ CASES) with "ENS2") as "[EN2 _]". *)
+(*           iPoseProof (OwnE_exploit with "[EN EN2]") as "%DIS". iFrame. *)
+(*           set_solver. *)
+(*       } *)
+(*       unfold lookup_def. rewrite CASES. ss. *)
+(*       iPoseProof ((OwnEs_acc_in _ _ _ CASES) with "ENS2") as "[EN2 ENS]". *)
+(*       iPoseProof (OwnE_union with "[EN EN2]") as "EN". iFrame. *)
+(*       iPoseProof (OwnEs_union with "[ENS EN]") as "ENS". iFrame. *)
+(*       replace (∅ ∪ (c0 ∪ E)) with (c0 ∪ E) by set_solver. *)
+(*       iModIntro. iFrame. *)
+(*     } *)
+(*     { replace (lookup_def Es1 n ∪ E) with (lookup_def Es1 n) by set_solver. *)
+(*       replace (lookup_def Es2 n ∪ E) with (lookup_def Es2 n) by set_solver. *)
+(*       rewrite insert_insert. *)
+(*       destruct (Es1 !! n) eqn:CASES. *)
+(*       - rewrite (insert_id Es1). *)
+(*         2:{ unfold lookup_def, default. rewrite CASES. ss. } *)
+(*         iPoseProof ("H" with "[A WSAT ENS]") as ">(A & WSAT & ENS2 & P)". iFrame. *)
+(*         iMod (OwnEs_lookup_def with "ENS2") as "ENS2". iModIntro. iFrame. *)
+(*       - replace (lookup_def Es1 n) with (⊤ : coPset). *)
+(*         2:{ unfold lookup_def, default. rewrite CASES. ss. } *)
+(*         iMod ((OwnEs_free _ _ CASES) with "ENS") as "ENS". *)
+(*         iPoseProof ("H" with "[A WSAT ENS]") as ">(A & WSAT & ENS2 & P)". iFrame. *)
+(*         iMod (OwnEs_lookup_def with "ENS2") as "ENS2". iModIntro. iFrame. *)
+(*     } *)
+(*   Qed. *)
+
+(*   Lemma FUpd_mask_frame x A Es1 Es2 n E1 E2 E P : *)
+(*     E1 ## E -> *)
+(*     FUpd x A (<[n:=E1]>Es1) (<[n:=E2]>Es2) P ⊢ *)
+(*          FUpd x A (<[n :=E1 ∪ E]>Es1) (<[n :=E2 ∪ E]>Es2) P. *)
+(*   Proof. *)
+(*     iIntros (D) "FUPD". *)
+(*     iPoseProof (FUpd_mask_frame_gen with "FUPD") as "FUPD". *)
+(*     { unfold lookup_def. rewrite lookup_insert. ss. eauto. } *)
+(*     unfold lookup_def. rewrite ! lookup_insert. ss. rewrite ! insert_insert. auto. *)
+(*   Qed. *)
+
+(*   Lemma FUpd_intro_mask x A Es1 Es2 Es3 n E1 E2 P : *)
+(*     E2 ⊆ E1 -> *)
+(*     FUpd x A (<[n:=E1]>Es1) (<[n:=E1]>Es2) P ⊢ *)
+(*          FUpd x A (<[n:=E1]>Es1) (<[n:=E2]>Es2) (FUpd x A (<[n:=E2]>Es3) (<[n:=E1]>Es3) P). *)
+(*   Proof. *)
+(*     rewrite /FUpd. iIntros (HE) "H (A & WSAT & ENS)". *)
+(*     iPoseProof ("H" with "[A WSAT ENS]") as ">(A & WSAT & ENS & P)". iFrame. *)
+(*     iModIntro. *)
+(*     rewrite (union_difference_L _ _ HE). *)
+(*     iPoseProof (OwnEs_disjoint with "ENS") as "[ENS EN]". *)
+(*     { set_solver. } *)
+(*     iFrame. iIntros "(A & WSAT & ENS)". iModIntro. iFrame. *)
+(*     iApply OwnEs_union. iFrame. *)
+(*   Qed. *)
+
+(*   Lemma FUpd_mask_mono x A Es1 Es2 n E1 E2 P : *)
+(*     E1 ⊆ E2 -> *)
+(*     FUpd x A (<[n:=E1]>Es1) (<[n:=E1]>Es2) P ⊢ FUpd x A (<[n:=E2]>Es1) (<[n:=E2]>Es2) P. *)
+(*   Proof. *)
+(*     i. replace E2 with (E1 ∪ E2 ∖ E1). *)
+(*     - eapply FUpd_mask_frame. set_solver. *)
+(*     - symmetry. eapply leibniz_equiv. eapply union_difference. ss. *)
+(*   Qed. *)
+
+(*   Global Instance from_modal_FUpd x A Es P : *)
+(*     FromModal True modality_id (FUpd x A Es Es P) (FUpd x A Es Es P) P. *)
+(*   Proof. *)
+(*     rewrite /FromModal /= /FUpd. iIntros. iModIntro. iFrame. iFrame. *)
+(*   Qed. *)
+
+(*   Global Instance from_modal_FUpd_general x A Es n E1 E2 P : *)
+(*     FromModal (E2 ⊆ E1) modality_id P (FUpd x A (<[n:=E1]>Es) (<[n:=E2]>Es) P) P. *)
+(*   Proof. *)
+(*     rewrite /FromModal /FUpd. ss. *)
+(*     iIntros (HE) "P (A & WSAT & EN)". iModIntro. iFrame. *)
+(*     iPoseProof (OwnEs_acc_in with "EN") as "[EN ENS]". apply lookup_insert. *)
+(*     iPoseProof ((OwnE_subset _ _ _ HE) with "EN") as "[EN1 _]". *)
+(*     iPoseProof (OwnEs_union with "[ENS EN1]") as "ENS". iFrame. rewrite insert_insert. *)
+(*     replace (∅ ∪ E2) with E2 by set_solver. iFrame. *)
+(*   Qed. *)
+
+(*   Global Instance from_modal_FUpd_wrong_mask x A Es1 Es2 P : *)
+(*     FromModal (pm_error "Only non-mask-changing update modalities can be introduced directly. *)
+(* Use [FUpd_mask_frame] and [FUpd_intro_mask]") *)
+(*               modality_id (FUpd x A Es1 Es2 P) (FUpd x A Es1 Es2 P) P | 100. *)
+(*   Proof. *)
+(*     intros []. *)
+(*   Qed. *)
+
+(*   Global Instance elim_modal_bupd_FUpd p x A Es1 Es2 P Q : *)
+(*     ElimModal True p false (|==> P) P (FUpd x A Es1 Es2 Q) (FUpd x A Es1 Es2 Q) | 10. *)
+(*   Proof. *)
+(*     rewrite /ElimModal bi.intuitionistically_if_elim /FUpd. *)
+(*     iIntros (_) "[P K] I". iMod "P". iApply ("K" with "P"). iFrame. *)
+(*   Qed. *)
+
+(*   Global Instance elim_modal_FUpd_FUpd p x A Es1 Es2 Es3 P Q : *)
+(*     ElimModal True p false (FUpd x A Es1 Es2 P) P (FUpd x A Es1 Es3 Q) (FUpd x A Es2 Es3 Q). *)
+(*   Proof. *)
+(*     rewrite /ElimModal bi.intuitionistically_if_elim /FUpd. *)
+(*     iIntros (_) "[P K] I". iMod ("P" with "I") as "(A & WSAT & EN & P)". *)
+(*     iApply ("K" with "P"). iFrame. *)
+(*   Qed. *)
+
+(*   Global Instance elim_modal_FUpd_FUpd_general p x A Es0 Es1 Es2 n E0 E1 E2 E3 P Q : *)
+(*     ElimModal (E0 ⊆ E2) p false *)
+(*               (FUpd x A (<[n:=E0]>Es0) (<[n:=E1]>Es1) P) *)
+(*               P *)
+(*               (FUpd x A (<[n:=E2]>Es0) (<[n:=E3]>Es2) Q) *)
+(*               (FUpd x A (<[n:=(E1 ∪ (E2 ∖ E0))]>Es1) (<[n:=E3]>Es2) Q) | 10. *)
+(*   Proof. *)
+(*     rewrite /ElimModal bi.intuitionistically_if_elim. ss. *)
+(*     iIntros (HE) "[M K]". *)
+(*     iPoseProof (FUpd_mask_frame _ _ _ _ _ _ _ (E2 ∖ E0) with "M") as "M". *)
+(*     { set_solver. } *)
+(*     replace (E0 ∪ E2 ∖ E0) with E2 by (eapply union_difference_L; ss). *)
+(*     iMod "M". iPoseProof ("K" with "M") as "M". iFrame. *)
+(*   Qed. *)
+
+(*   Global Instance elim_acc_FUpd *)
+(*          {X : Type} i A Es1 Es2 Es (α β : X -> iProp) (mγ : X -> option iProp) (Q : iProp) : *)
+(*     ElimAcc True (FUpd i A Es1 Es2) (FUpd i A Es2 Es1) α β mγ (FUpd i A Es1 Es Q) (fun x : X => ((FUpd i A Es2 Es2 (β x)) ∗ (mγ x -∗? FUpd i A Es1 Es Q))%I). *)
+(*   Proof. *)
+(*     iIntros (_) "Hinner >[% [Hα Hclose]]". *)
+(*     iPoseProof ("Hinner" with "Hα") as "[>Hβ Hfin]". *)
+(*     iPoseProof ("Hclose" with "Hβ") as ">Hγ". *)
+(*     iApply "Hfin". iFrame. *)
+(*   Qed. *)
+
+(*   Global Instance into_acc_FUpd_inv x A Es n N P : *)
+(*     IntoAcc (inv n N P) (n < x /\ subseteq_def Es n (↑N)) True *)
+(*             (FUpd x A Es (<[n := lookup_def Es n ∖ ↑N]>Es)) *)
+(*             (FUpd x A (<[n := lookup_def Es n ∖ ↑N]>Es) Es) *)
+(*             (fun _ : () => P) (fun _ : () => P) (fun _ : () => None). *)
+(*   Proof. *)
+(*     rewrite /IntoAcc. iIntros ((LT & iE)) "INV _". rewrite /accessor. *)
+(*     iPoseProof (FUpd_open _ _ _ _ _ LT iE with "INV") as ">[open close]". *)
+(*     iModIntro. iExists tt. iFrame. *)
+(*   Qed. *)
+
+(*   Global Instance elim_modal_iupd_FUpd p x A Es1 Es2 P Q : *)
+(*     ElimModal True p false (#=(A)=> P) P (FUpd x A Es1 Es2 Q) (FUpd x A Es1 Es2 Q) | 10. *)
+(*   Proof. *)
+(*     rewrite /ElimModal bi.intuitionistically_if_elim /FUpd. *)
+(*     iIntros (_) "[P K] [A I]". *)
+(*     iMod ("P" with "A") as "[A P]". iApply ("K" with "P"). iFrame. *)
+(*   Qed. *)
+
+(* End FANCY_UPDATE. *)
+
+(* Global Opaque FUpd. *)
 
 (* Section FANCY_UPDATE. *)
 
